# Summary of the Differential Equation and Solution

## Initial Conditions:
- \( y(0) = 0 \) (initial value of \( y \) when \( x = 0 \))
- \( x(0) = 0 \) (initial value of \( x \))

## Differential Equation:
The differential equation is:

\[
\frac{dy}{dx} = y + x
\]

## Solution:
The general solution to the differential equation is:

\[
y(x) = -x + 1 + C e^{x}
\]

Using the initial condition \( y(0) = 0 \), we find that \( C = -1 \). Thus, the specific solution becomes:

\[
y(x) = -x + 1 - e^{x}
\]

## Evaluation:
At \( x = 1 \):

\[
y(1) = -1 + 1 - e = -e \approx -2.718
\]
